WIP

proof/SimMod.v
@@ -14,7 +14,7 @@ Require Import LinkingC.
 
 Require Import Syntax Sem Mod ModSem.
 Require Import Sound.
-Require Import SimSymb SimMem SimModSem.
+Require Import SimSymb SimMem SimModSemUnified.
 
 Set Implicit Arguments.
 
@@ -36,11 +36,7 @@ Context `{SM: SimMem.class} {SS: SimSymb.class SM} {SU: Sound.class}.
   }.
 
   Definition to_msp (midx: Midx.t)
-             (skenv_link_src skenv_link_tgt: SkEnv.t) (sm: SimMem.t) (mp: t)
-             (SMO: SimMemOh.class
-                     ((Mod.modsem (mp.(src)) midx skenv_link_src).(ModSem.owned_heap))
-                     ((Mod.modsem (mp.(tgt)) midx skenv_link_tgt).(ModSem.owned_heap)))
-    : ModSemPair.t
+             (skenv_link_src skenv_link_tgt: SkEnv.t) (sm: SimMem.t) (mp: t): ModSemPair.t
     := ModSemPair.mk (Mod.modsem (mp.(src)) midx skenv_link_src)
                      (Mod.modsem (mp.(tgt)) midx skenv_link_tgt) mp.(ss) sm.
 
@@ -60,7 +56,8 @@ Context `{SM: SimMem.class} {SS: SimSymb.class SM} {SU: Sound.class}.
           (SIMSKENVLINK: SimSymb.sim_skenv sm_init_link ss_link skenv_link_src skenv_link_tgt),
           exists SMO, <<SIMMSP: ModSemPair.sim
                                   (to_msp midx skenv_link_src skenv_link_tgt
-                                          sm_init_link mp SMO)>>).
+                                          sm_init_link mp)
+                                  (SMO := SMO)>>).
   (* TODO: quantifying "exists SMO" here looks somewhat dirty... *)
   (* I would like to quantify it directly inside "sim_intro", but I need to put it here because *)
   (* I need to know "owned_heap" type which needs to know "skenv_link_src,tgt". *)
@@ -69,6 +66,21 @@ Context `{SM: SimMem.class} {SS: SimSymb.class SM} {SU: Sound.class}.
   (* TODO: the same goes for "state" too. *)
 
   (* Design: ModPair only has data, properties are stated in sim *)
+
+  Inductive simU {SMOS: SimMemOhs.class} (mp: t): Prop :=
+  | simU_intro
+      (SIMSK: SimSymb.wf mp.(ss))
+      (SKSRC: mp.(ss).(SimSymb.src) = (Mod.sk mp.(src)))
+      (SKTGT: mp.(ss).(SimSymb.tgt) = (Mod.sk mp.(tgt)))
+      (SIMMS: forall midx skenv_link_src skenv_link_tgt ss_link sm_init_link
+          (INCLSRC: SkEnv.includes skenv_link_src (Mod.sk mp.(src)))
+          (INCLTGT: SkEnv.includes skenv_link_tgt (Mod.sk mp.(tgt)))
+          (WFSRC: SkEnv.wf skenv_link_src)
+          (WFTGT: SkEnv.wf skenv_link_tgt)
+          (SSLE: SimSymb.le mp.(ss) ss_link)
+          (SIMSKENVLINK: SimSymb.sim_skenv sm_init_link ss_link skenv_link_src skenv_link_tgt),
+          <<SIMMSP: ModSemPair.simU (to_msp midx skenv_link_src skenv_link_tgt
+                                            sm_init_link mp)>>).
 
 End MODPAIR.
 End ModPair.
